formalization/thesis/Isotope/LambdaIter/Named.lean
@@ -6,5 +6,7 @@ import Isotope.LambdaIter.Named.Subtyping
 import Isotope.LambdaIter.Named.Typing
 import Isotope.LambdaIter.Named.Structural
 import Isotope.LambdaIter.Named.Subst
+import Isotope.LambdaIter.Named.Alpha
 import Isotope.LambdaIter.Named.Equiv
+import Isotope.LambdaIter.Named.EquivStructural
 import Isotope.LambdaIter.Named.Examples
